checkpoint for example-4

fatnode/FatNode.dfy
@@ -1,309 +1,67 @@
-// class Entry {
-//   ghost var Repr: set<Node>
-
-//   var roots: seq<Node?>
-//   var time: int
-
-//   predicate Valid()
-//     reads this, Repr
-//   {
-//     time >= 0 && |roots| > 0 &&
-//     (forall r :: r in roots && r != null ==> r in Repr && Repr >= r.Repr && r.Valid()) // it is a bit weird not being able to write only "Repr >= r.Repr && r.Valid()""
-//   }
-
-//   constructor Init()
-//     ensures Valid()
-//   {
-//     roots := [null];
-//     time := 0;
-//     Repr := {};
-//   }
-  
-//   // method Insert(value: int)
-//   //   requires Valid()
-//   //   modifies this, Repr
-//   //   ensures Valid()
-//   // {
-//   //   time := time + 1;
-//   //   var root := roots[|roots| - 1];
-//   //   if root == null {
-//   //     var node := new Node.Init(time, value);
-//   //     roots := roots + [node];
-//   //     Repr := Repr + {node};
-//   //     assert Repr >= node.Repr;
-//   //   } else {
-//   //     var newNode := root.Insert(time, value);
-//   //     roots := roots + [root];
-//   //     Repr := Repr + {newNode} + newNode.Repr;
-//   //     assert Repr >= newNode.Repr;
-//   //   }
-//   // }
-// }
-
-
 class Node {
   ghost var Repr: set<Node>
+  ghost var ValueSets: seq<(int, set<int>)> 
 
+  var created: int
+  var removed: int
+  var value: int
   var lefts: seq<(int, Node?)>
   var rights: seq<(int, Node?)>
-  var values: seq<(int, int)>
+  var data: seq<(int, int)>
 
+  // Consistently use A && B ==> C when I wrote A ==> B ==> C
   predicate Valid()
     reads this, Repr
+    ensures Valid() ==> this in Repr
   {
-    |values| > 0 &&
-    this in Repr &&
-    (forall l :: l in lefts && l.1 != null ==> 
-      l.1 in Repr && l.1.Repr < Repr && this !in l.1.Repr && l.1.Valid()) &&
-    (forall r :: r in rights && r.1 != null ==> 
-      r.1 in Repr && r.1.Repr < Repr && this !in r.1.Repr && r.1.Valid()) &&
-    (forall r, l :: r in rights && l in lefts && r.1 != null && l.1 != null ==>
-      l.1 != r.1 && l.1.Repr !! r.1.Repr) && // needed to add l.0 != r.0 
-    // (forall i, j :: 0 <= i < j < |lefts| ==> lefts[i].0 < lefts[j].0) &&
-    // (forall i, j :: 0 <= i < j < |rights| ==> rights[i].0 < rights[j].0) &&
-    // (forall i, j :: 0 <= i < j < |values| ==> values[i].0 < values[j].0) 
-    // COMMENT: The following does not hold due to the delete method
-    (forall r1, r2 :: r1 in rights && r2 in rights && r1.1 != null && r2.1 != null  ==>
-      r1 != r2 ==> r1.1.Repr !! r2.1.Repr) &&
-    (forall l1, l2 :: l1 in lefts && l2 in lefts && l1.1 != null && l2.1 != null ==>
-      l1 != l2 ==> l1.1.Repr !! l2.1.Repr)
-  } 
-
-  constructor Init(time: int, value: int)
-    ensures Valid() && fresh(Repr)
-    ensures lefts == []
-    ensures rights == []
-    ensures Repr == {this}
-    ensures values == [(time, value)]
-  {
-    lefts := [];
-    rights := [];
-    values := [(time, value)];
-    Repr := {this};
+    created >= 0 
+    && (removed == -1 || removed > created) 
+    && |data| > 0 
+    && |ValueSets| >= |data|
+    && data[0].0 == created 
+    && ValueSets[0].0 == created
+    && |ValueSets[0].1| == 1
+    && this in Repr
+    && (forall l <- lefts | l.1 != null ::
+      l.1 in Repr && this !in l.1.Repr && l.1.Repr < Repr && l.1.Valid()) 
+    && (forall r <- rights | r.1 != null ::
+      r.1 in Repr && this !in r.1.Repr && r.1.Repr < Repr &&r.1.Valid()) 
+    && (forall r <- rights, l <- lefts | r.1 != null && l.1 != null :: 
+      l.1 != r.1 && l.1.Repr !! r.1.Repr && l.0 != r.0) 
+    && (forall i, j | 0 <= i < j < |lefts| :: created < lefts[i].0 < lefts[j].0) 
+    && (forall i, j | 0 <= i < j < |rights| :: created < rights[i].0 < rights[j].0) 
+    && (forall i, j | 0 <= i < j < |data| :: created <= data[i].0 < data[j].0)
+    && (forall i, j | 0 <= i < j < |ValueSets| :: created <= ValueSets[i].0 < ValueSets[j].0) 
+    && (forall i | 0 <= i < |ValueSets| :: ValueSets[i].0 >= created) 
+    && (forall i | 0 <= i < |data| :: data[i].0 >= created)
+    && (forall i | 0 <= i < |lefts| :: lefts[i].0 > created)
+    && (forall i | 0 <= i < |rights| :: rights[i].0 > created)
+    && (removed > 0 ==>
+        && (forall i | 0 <= i < |lefts| :: lefts[i].0 < removed) 
+        && (forall i | 0 <= i < |rights| :: rights[i].0 < removed) 
+        && (forall i | 0 <= i < |data| :: data[i].0 < removed)) 
+    // data and ValueSets
+    && (forall timedValueSet <- ValueSets ::  
+        created <= timedValueSet.0 && (removed == -1 || timedValueSet.0 <= removed)) 
+    && (forall timedValueSet <- ValueSets, node <- Repr, childTimedValueSet <- node.ValueSets :: 
+        childTimedValueSet.0 <= timedValueSet.0 ==> childTimedValueSet.1 <= timedValueSet.1) 
+    && (forall i | 0 <= i < |data| :: 
+          exists j | i <= j < |ValueSets| :: 
+            ValueSets[j].0 == data[i].0 && data[i].1 in ValueSets[j].1)
   }
 
-  function method Left(): (l: Node?)
-    reads Repr 
-    requires Valid()
-    ensures |values| > 0
-    ensures l != null ==> l.Valid()
-  {
-    if |lefts| > 0 then
-      lefts[|lefts| - 1].1
-    else
-      null
-  }
-
-  function method Right(): (r: Node?)
-    reads Repr 
-    requires Valid()
-    ensures r != null ==> r.Valid()
-  {
-    if |rights| > 0 then
-      rights[|rights| - 1].1
-    else
-      null
-  }
-
-  function method Value(): int
-    reads Repr 
-    requires Valid()
-  {
-    values[|values| - 1].1
-  }
-
-  function method ValueVersions(s: seq<(int, int)>): seq<int>
-  {
-    seq(|s|, i requires 0 <= i < |s| => s[i].0)
-  }
-
-  function method NodeVersions(s: seq<(int, Node?)>): seq<int>
-  {
-    seq(|s|, i requires 0 <= i < |s| => s[i].0)
-  }
-
-  function method BinarySearch(v: int, s: seq<int>, lo: int, hi: int): (index: int)
-    requires |s| - 1 >= hi
-    requires 0 <= lo <= hi + 1
-    decreases hi - lo
-    ensures -1 <= index < |s|
-  {
-    if |s| == 0 || v < s[0] || lo > hi then
-      -1
-    else
-      var mid := lo + (hi - lo) / 2;
-      var v' := s[mid];
-      if v > v' then
-        BinarySearch(v, s, mid + 1, hi)
-      else if v < v' then
-        BinarySearch(v, s, lo, mid - 1)
-      else
-        mid
-  }
-
-  function method FindValue(version: int): (bool, int)
-    requires Valid()
-    reads Repr 
-  {
-    var i := BinarySearch(version, ValueVersions(values), 0, |values| - 1);
-    if i == -1 then
-      (false, -1)
-    else
-      (true, values[i].1)
-  }
-
-  function method FindNode(version: int, left: bool): Node?
-    requires Valid()
-    reads Repr 
-  {
-    if left then
-      var i := BinarySearch(version, NodeVersions(lefts), 0, |lefts| - 1);
-      if i == -1 then
-        null
-      else
-        lefts[i].1
-    else
-      var i := BinarySearch(version, NodeVersions(rights), 0, |rights| - 1);
-      if i == -1 then
-        null
-      else
-        rights[i].1
-  }
-
-  function method Find(version: int, value: int): bool
-    requires Valid()
+  function ValueSetVersions(): (res: seq<int>)
     reads Repr
-  {
-    var (found, x) := FindValue(version);
-    if found then
-      if x > Value() then
-        var left := FindNode(version, true);
-        if left == null then
-          false
-        else
-          left.Find(version, value)
-      else if x < Value() then
-        var right := FindNode(version, false);
-        if right == null then
-          false
-        else
-          right.Find(version, value)
-      else
-        true
-    else
-      false
-  }
-
-  method Insert(time: int, value: int) returns (node: Node?)
     requires Valid()
-    // requires time > maxTime
-    modifies Repr
-    decreases Repr
-    ensures |values| > 0
-    ensures node == null ==> 
-      Repr == old(Repr)
-    ensures node != null ==> 
-      fresh(node) &&
-      node.Repr == {node} && 
-      // node.lefts == [] && node.rights == [] &&
-      Repr == old(Repr) + {node} 
     ensures Valid()
-  {
-    var x := Value();
-    if x < value {
-      var r := Right();
-      if r == null {
-        node := new Node.Init(time, value);
-        rights := rights + [(time, node)];
-        Repr := Repr + node.Repr;
-      } else {
-        node := r.Insert(time, value);
-        if (node != null) {
-          Repr := Repr + node.Repr;
-        } 
-      }
-    } else if x > value {
-      var l := Left();
-      if l == null {
-        node := new Node.Init(time, value);
-        lefts := lefts + [(time, node)];
-        Repr := Repr + node.Repr;
-      } else {
-        node := l.Insert(time, value);
-        if (node != null) {
-          Repr := Repr + node.Repr;
-        }
-      }
-    } else {
-      node := null;
-    }
+    // COMMENT: This assertion is literally part of Valid()
+    ensures forall i | 0 <= i < |data| :: 
+             exists j | i <= j < |ValueSets| :: 
+              ValueSets[j].0 == data[i].0 && data[i].1 in ValueSets[j].1
+  { 
+    seq(|ValueSets|, i requires 0 <= i < |ValueSets| 
+                    requires Valid()
+                    reads this, Repr => 
+                    ValueSets[i].0)
   }
-
-  // method DeleteMin(parent: Node, fromLeft: bool, time: int) returns (minV: int)
-  //   requires Valid() && parent.Valid()
-  //   requires parent.Left() == this || parent.Right() == this
-  //   decreases Repr
-  //   modifies parent.Repr
-  //   ensures lefts == old(lefts)
-  //   // ensures rights == old(rights)
-  //   ensures parent.Valid()
-  // {
-  //   var l := Left();
-  //   if l == null {
-  //     assert Valid();
-  //     if fromLeft {
-  //       parent.lefts := parent.lefts + [(time, Right())];
-  //     } else {
-  //       parent.rights := parent.rights + [(time, Right())];
-  //     }
-  //     assert Valid();
-  //     assert parent.Valid();
-  //     minV := Value();
-  //     assert parent.Valid();
-  //     assert lefts == old(lefts);
-  //   } else {
-  //     assert Valid();
-  //     minV := l.DeleteMin(this, true, time);
-  //     assert lefts == old(lefts);
-  //     assert Valid();
-  //     // assert parent.Valid();
-  //   }
-  // }
-
-  // method Delete(parent: Node?, fromLeft: bool, time: int, value: int) returns (root: Node?) 
-  //   requires Valid()
-  //   modifies Repr
-  //   decreases Repr
-  //   ensures root != null ==> root.Valid()
-  // {
-  //   var x := Value();
-  //   var r := Right();
-  //   var l := Left();
-  //   if x == value {
-  //     if r != null {
-  //       var minV := r.DeleteMin(this, false, time);
-  //       values := values + [(time, minV)];
-  //     } else {
-  //       if parent != null {
-  //         if fromLeft {
-  //           lefts := lefts + [(time, l)];
-  //         } else {
-  //           rights := rights + [(time, l)];
-  //         }
-  //       } else {
-  //         root := l;
-  //       }
-  //     }
-  //   } else if x < value {
-  //     if r != null {
-  //       root := r.Delete(this, false, time, value);
-  //     }
-  //   } else {
-  //     if l != null {
-  //       root := l.Delete(this, true, time, value);
-  //     }
-  //   }
-
-  //   root := this;
-  // }
 }
